(wip) Global translation

Translation/Global.lean
@@ -5,15 +5,29 @@ import Surface.Typing
 
 import Translation.Ty
 
+def Core.is_valid_ctor_ty (G : Core.GlobalEnv) : Core.Ty -> Option Unit
+| .all _ T => is_valid_ctor_ty G T
+| .arrow _ T => is_valid_ctor_ty G T
+| t => do let (x, _) <- t.spine
+          if Core.is_data G x then return () else none
+
+def Surface.Ty.translate_ctors (G : Core.GlobalEnv) (ctors : Vect n  (String × Surface.Ty)) : Option (Vect n (String × Core.Ty)) := do
+  -- check that names are unique
+  let cns : Vect n String := (λ x => x.1) <$> ctors
+
+  let octors' : Vect n (Option (String × Core.Ty)) :=  (λ (x, ty) =>
+    do let ty' : Core.Ty <- ty.translate
+       let _ <- Core.is_valid_ctor_ty G ty'
+       return (x , ty')) <$> ctors
+  octors'.seq
+
+
+
 @[simp]
-def Surface.Global.translate (_ : Core.GlobalEnv) : Global -> Option Core.Global
+def Surface.Global.translate (G : Core.GlobalEnv) : Global -> Option Core.Global
 | .data (n := n) x K ctors => do
-  let K' := K.translate
-  let octors' : Vect n (Option (String × Core.Ty)) :=  λ i =>
-    do let ty' : Core.Ty <- (ctors i).2.translate
-       return ((ctors i).1 , ty')
-  let ctors' <- octors'.seq
-  return Core.Global.data n x K' ctors'
+  let ctors' <- Ty.translate_ctors G ctors
+  return Core.Global.data n x K.translate ctors'
 
 @[simp]
 def Surface.GlobalEnv.translate : Surface.GlobalEnv -> Option (Core.GlobalEnv)
